Spqr.lean
@@ -1,3 +1,5 @@
+import Spqr.Aux.Aeneas.StdNextCoreIterRangeStep
+import Spqr.Aux.Aeneas.StdNextStepUsize
 import Spqr.Code.Funs
 import Spqr.Code.FunsExternal
 import Spqr.Code.Types
@@ -13,6 +15,7 @@ import Spqr.Specs.Encoding.Gf.GF16.AddAssign
 import Spqr.Specs.Encoding.Gf.GF16.ConstDiv
 import Spqr.Specs.Encoding.Gf.GF16.ConstMul
 import Spqr.Specs.Encoding.Gf.GF16.ConstSub
+import Spqr.Specs.Encoding.Gf.GF16.DivImpl
 import Spqr.Specs.Encoding.Gf.GF16.Eq
 import Spqr.Specs.Encoding.Gf.GF16.Mul
 import Spqr.Specs.Encoding.Gf.GF16.MulAssign
